Use equations plugin

theories/const.v
@@ -4,17 +4,24 @@ Require Import FunInd.
 Require Import Lia.
 Require Import Coq.Program.Tactics.
 
+From Equations Require Import Equations.
+
 Import CPS.
 
 (** [in_map l f] is just like [map f l] except that the function carries a proof
     that its argument is an element of [l]. *)
-Program Fixpoint in_map {A B: Type} (l: list A) (f: {a: A | In a l} -> B) : list B :=
-    match l with 
-    | a :: tl => (f a) :: (in_map tl f)
-    | _ => nil
-    end.
-Next Obligation. simpl. left. reflexivity. Qed.
-Next Obligation. simpl. right. auto. Qed.
+Equations in_map {A B: Type} (l: list A) (f: forall (e: A), In e l -> B) : list B :=
+    | a :: tl, f => (f a _) :: (in_map tl (fun e H => f e _))
+    | _, _ => nil.
+
+Lemma in_map_length: forall A B (l: list A) (f: forall (e: A), In e l -> B),
+    length (in_map l f) = length l.
+Proof.
+    intros. induction l.
+    - trivial.
+    - simpl. autorewrite with in_map. simpl. rewrite IHl. trivial.
+Qed.
+
 
 Lemma list_max_in: forall e l, In e l -> e <= list_max l.
 Proof.
@@ -31,11 +38,11 @@ Qed.
 Lemma Nlt_succ_le: forall n m, n < S m <-> n <= m.
 Proof. lia. Qed.
 
+
 (** [const_fold exp] is [exp] with operations of the form
     [n_1 op n_2] or [op n] folded with their values substituted into
     their uses. *)
-Program Fixpoint const_fold (exp: cexp) {measure (depth exp)} : cexp :=
-    match exp with
+Equations const_fold (exp: cexp) : cexp by wf (depth exp) Nat.lt :=
     | cbop op (i64 lhs) (i64 rhs) k =>
         cbop op (i64 lhs) (i64 rhs) (const_fold (substitute O (i64 (bop_eval op lhs rhs)) k))
     | cbop op lhs rhs k => cbop op lhs rhs (const_fold k)
@@ -43,32 +50,31 @@ Program Fixpoint const_fold (exp: cexp) {measure (depth exp)} : cexp :=
         cuop op (i64 v) (const_fold (substitute O (i64 (uop_eval op v)) k))
     | cuop op b k => cuop op b (const_fold k)
     | capp x y => capp x y
-    | cfix fns k => cfix (in_map fns (fun (e: {a: string * nat * cexp | In a fns}) => 
-                                      let '(a, b, k) := e in 
-                                        (a, b, const_fold k))) 
+    | cfix fns k => cfix (in_map fns (fun e H => 
+                                      let '(a, b, _) := e in 
+                                        (a, b, const_fold (snd e)))) 
                     (const_fold k)
-    | csel c branches => csel c (in_map branches (fun br => const_fold br))
+    | csel c branches => csel c (in_map branches (fun br H => const_fold br))
     | ceff op args k => ceff op args (const_fold k)
-    | fin => fin
-    end.
+    | fin => fin.
 Next Obligation.
 rewrite <- subst_preserve_depth with (n := O) (v := i64 (bop_eval op lhs rhs)). auto.
 Qed.
 Next Obligation.
 rewrite <- subst_preserve_depth with (n := O) (v := i64 (uop_eval op v)). auto.
 Qed.
-Next Obligation. simpl. rewrite Nlt_succ_le. apply Nat.max_le_iff.
+Next Obligation.
+    simpl. rewrite Nlt_succ_le. apply Nat.max_le_iff.
     left. apply list_max_in. 
-    change (depth c) with ((fun '(_, _, b) => depth b) (s, n, c)).
+    change (depth c0) with ((fun '(_, _, b) => depth b) (s0, n0, c0)).
     apply List.in_map. assumption. Qed.
 Next Obligation. simpl. auto with arith. Qed.
 Next Obligation. simpl. rewrite Nlt_succ_le. apply list_max_in. apply List.in_map.
 assumption. 
 Defined.
 
-Definition matches s_1 s_2 := s_1.(tr) = s_2.(tr).
 
-Ltac psimpl f := unfold f; rewrite fix_sub_eq; simpl; fold f.
+Definition matches s_1 s_2 := s_1.(tr) = s_2.(tr).
 
 Fixpoint const_fold_fuel (exp: cexp) (fuel: nat): cexp :=
     match (fuel, exp) with
@@ -98,8 +104,7 @@ Qed.
 
 
 
-(* TODO: Is this statement actually proving what we want it to prove? *)
-Theorem const_lock_sim: forall c c' s_1 s_2 s_1' n,
+Theorem const_fuel_lock_single: forall c c' s_1 s_2 s_1' n,
     matches s_1 s_2 -> small_step c s_1 c' s_1' -> n > depth c ->
     (exists c_2' s_2', small_step (const_fold_fuel c n) s_2 c_2' s_2' /\ matches s_1' s_2').
 Proof.
@@ -116,9 +121,53 @@ Proof.
     - unfold matches. unfold matches in H. now rewrite H.
 Qed.    
 
-(* Theorem const_fold_eq: forall n c, n > depth c -> const_fold_fuel c n = const_fold c.
+Lemma const_lock_single: forall c c' s_1 s_2 s_1',
+    matches s_1 s_2 -> small_step c s_1 c' s_1' ->
+    (exists c_2' s_2', small_step (const_fold c) s_2 c_2' s_2' /\ matches s_1' s_2').
 Proof.
-    induction n.
-    - intros. inversion H.
-    - intros. simpl. destruct c.
-        +    *)
+    intros. destruct H0.
+    all: eexists; eexists; split; (assumption || autorewrite with const_fold; simpl; auto).
+    (* Select *)
+    - autorewrite with const_fold. apply ssel. destruct H0. split.
+        * now rewrite in_map_length.
+        * assumption.
+    (* Select case 2 *)
+    - assumption.
+    (* Effect *)
+    - unfold matches. unfold matches in H. now rewrite H.
+Qed.
+
+(* I don't think this is right... *)
+Inductive lock_matches: cexp -> State -> cexp -> State -> Prop :=
+    | lock_matches_intro: forall c_1 s_1 c_2 s_2, 
+        matches s_1 s_2 -> 
+        c_2 = const_fold c_1 -> 
+        lock_matches c_1 s_1 c_2 s_2
+    | lock_matches_step: forall c_1 s_1 c_2 s_2 c_1' s_1' c_2' s_2', 
+        lock_matches c_1 s_1 c_2 s_2 ->
+        small_step c_1 s_1 c_1' s_1' ->
+        small_step c_2 s_2 c_2' s_2' ->
+        matches s_1' s_2' ->
+        lock_matches c_1' s_1' c_2' s_2'.
+
+(* Or this... *)
+Theorem const_lock_simulation: forall c_1 s_1 c_1' s_1' c_2 s_2,
+    lock_matches c_1 s_1 c_2 s_2 -> small_step c_1 s_1 c_1' s_1' -> 
+    (exists c_2' s_2', small_step c_2 s_2 c_2' s_2' /\ lock_matches c_1' s_1' c_2' s_2').
+Proof.
+    intros. induction H.
+    - pose proof H0 as H'. apply const_lock_single with (s_2 := s_2) in H0; auto.
+        destruct H0 as (c_2' & s_2' & H0 & H0'). 
+        rewrite <- H1 in H0. exists c_2'. exists s_2'. split.
+        + apply H0.
+        + apply lock_matches_step with (c_1 := c_1) (s_1 := s_1) (c_2 := c_2) (s_2 := s_2); auto.
+            apply lock_matches_intro; auto.
+    - rename c_1' into c_1''. rename s_1' into s_1''. rename c_1'0 into c_1'. rename s_1'0 into s_1'.
+        Admitted.
+    (* intros. inversion H.
+    - pose proof H0 as H'. apply const_lock_single with (s_2 := s_2) in H0; auto.
+        destruct H0 as (c_2' & s_2' & H0 & H0'). 
+        rewrite <- H2 in H0. exists c_2'. exists s_2'. split.
+        + apply H0.
+        + apply lock_matches_step with (c_1 := c_1) (s_1 := s_1) (c_2 := c_2) (s_2 := s_2); auto.
+    -  *)
